Compiler/Erase.v
@@ -201,7 +201,9 @@ Section CompatibilityLemmas.
     (* destruct assumptions *)
     intros vr₁ vr₂.
     rewrite -> valrel_fixp in vr₁.
-    destruct vr₁ as [ot [tsb [tub [eq₁ [eq₂ bodyrel]]]]]; subst.
+    destruct vr₁ as [ot hyp]; subst; cbn in hyp.
+    apply OfType_inversion_ptarr in ot.
+    destruct ot as (tsb & tub & eqs & equ & _); subst.
     destruct (valrel_implies_Value vr₂) as [vvs₂ vvu₂].
 
     (* beta-reduce *) 
@@ -217,7 +219,7 @@ Section CompatibilityLemmas.
     refine (termrel_antired w es1 eu1 _ _ _); unfold lev in *; simpl; try omega.
 
     (* use assumption for function body *)
-    eapply bodyrel; try omega; eauto using valrel_mono.
+    eapply hyp; try omega; eauto using valrel_mono.
   Qed.    
     
 
@@ -344,8 +346,13 @@ Section CompatibilityLemmas.
 
     (* then evaluate the projection *)
     rewrite -> valrel_fixp in H.
-    destruct H as [ot [vs₁ [vs₂ [vu₁ [vu₂ [? [? [vr₁ vr₂]]]]]]]]; subst.
-    destruct (OfType_implies_Value ot) as [[vvs₁ vvs₂] [vvu₁ vvu₂]].
+    destruct H as [ot hyp]; subst; cbn in hyp.
+    apply OfType_inversion_ptprod in ot.
+    destruct ot as (vs₁ & vu₁ & vs₂ & vu₂ & ? & ? & ot₁ & ot₂); subst.
+    destruct (OfType_implies_Value ot₁) as [vvs₁ vvs₂].
+    destruct (OfType_implies_Value ot₂) as [vvu₁ vvu₂].
+    destruct hyp as [vr₁ vr₂].
+
     assert (S.eval (S.proj₂ (S.pair vs₁ vs₂)) vs₂) by 
         (apply (S.eval_ctx₀ S.phole); try refine (S.eval_proj₂ _ _); simpl; intuition).
     assert (esn : S.evaln (S.proj₂ (S.pair vs₁ vs₂)) vs₂ 1) by eauto using S.evaln.
@@ -380,8 +387,13 @@ Section CompatibilityLemmas.
 
     (* then evaluate the projection *)
     rewrite -> valrel_fixp in H.
-    destruct H as [ot [vs₁ [vs₂ [vu₁ [vu₂ [? [? [vr₁ vr₂]]]]]]]]; subst.
-    destruct (OfType_implies_Value ot) as [[vvs₁ vvs₂] [vvu₁ vvu₂]].
+    destruct H as [ot hyp]; subst; cbn in hyp.
+    apply OfType_inversion_ptprod in ot.
+    destruct ot as (vs₁ & vu₁ & vs₂ & vu₂ & ? & ? & ot₁ & ot₂); subst.
+    destruct (OfType_implies_Value ot₁) as [vvs₁ vvs₂].
+    destruct (OfType_implies_Value ot₂) as [vvu₁ vvu₂].
+    destruct hyp as [vr₁ vr₂].
+
     assert (S.eval (S.proj₁ (S.pair vs₁ vs₂)) vs₁) by 
         (apply (S.eval_ctx₀ S.phole); try refine (S.eval_proj₁ _ _); simpl; intuition).
     assert (esn : S.evaln (S.proj₁ (S.pair vs₁ vs₂)) vs₁ 1) by eauto using S.evaln.
@@ -450,8 +462,8 @@ Section CompatibilityLemmas.
 
   Lemma termrel_caseof {d w τ τ₁ τ₂ ts₁ ts₂ ts₃ tu₁ tu₂ tu₃} :
     termrel d w (ptsum τ₁ τ₂) ts₁ tu₁ →
-    (forall w' vs₁ vu₁, w' ≤ w → valrel d w' τ₁ vs₁ vu₁ → termrel d w' τ (ts₂ [beta1 vs₁]) (tu₂ [ beta1 vu₁])) →
-    (forall w' vs₂ vu₂, w' ≤ w → valrel d w' τ₂ vs₂ vu₂ → termrel d w' τ (ts₃ [beta1 vs₂]) (tu₃ [ beta1 vu₂])) →
+    (forall w' vs₁ vu₁, w' < w → valrel d w' τ₁ vs₁ vu₁ → termrel d w' τ (ts₂ [beta1 vs₁]) (tu₂ [ beta1 vu₁])) →
+    (forall w' vs₂ vu₂, w' < w → valrel d w' τ₂ vs₂ vu₂ → termrel d w' τ (ts₃ [beta1 vs₂]) (tu₃ [ beta1 vu₂])) →
     termrel d w τ (S.caseof ts₁ ts₂ ts₃) (U.caseof tu₁ tu₂ tu₃).
   Proof.
     intros tr₁ tr₂ tr₃.
@@ -463,8 +475,11 @@ Section CompatibilityLemmas.
 
     (* then evaluate the caseof *)
     rewrite -> valrel_fixp in H.
-    destruct H as [ot [[vs' [vu' [? [? vr]]]]|[vs' [vu' [? [? vr]]]]]]; subst;
-    destruct (OfType_implies_Value ot) as [vvs vvu]; clear ot.
+    destruct H as [ot hyp]; subst; cbn in hyp.
+    apply OfType_inversion_ptsum in ot.
+    destruct ot as (vs' & vu' & [(? & ? & ot)|[(? & ?)|[(? & ?)|(? & ? & ot)]]]);
+      subst; cbn in *; try contradiction;
+      destruct (OfType_implies_Value ot) as [vvs vvu]; clear ot.
     - assert (S.eval (S.caseof (S.inl vs') ts₂ ts₃) (ts₂ [beta1 vs'])) by
           (apply (S.eval_ctx₀ S.phole); try refine (S.eval_case_inl _); simpl; intuition).
       assert (esn : S.evaln (S.caseof (S.inl vs') ts₂ ts₃) (ts₂ [beta1 vs']) 1) by eauto using S.evaln.
@@ -511,12 +526,12 @@ Section CompatibilityLemmas.
     
     (* destruct valrel assumption *)
     intros vr.
-    destruct (valrel_implies_Value vr) as [vvs vvu].
     rewrite -> valrel_fixp in vr.
-    destruct vr as [ot [tsb [tub [? [? bodyrel]]]]]; subst.
+    destruct vr as [ot hyp]; cbn in hyp. crush.
+    destruct ot as (tsb & tub & ? & ? & ?); crush.
 
     (* evaluate *)
-    assert (es : S.fixt (repEmul τ₁) (repEmul τ₂) (S.abs (repEmul (ptarr τ₁ τ₂)) tsb) --> tsb [beta1 (S.abs (repEmul τ₁) (S.app (S.fixt (repEmul τ₁) (repEmul τ₂) (S.abs (repEmul τ₁ ⇒ repEmul τ₂) tsb[wkm↑])) (S.var 0)))]) by (refine (eval_ctx₀ S.phole _ _); crush).
+    assert (es : S.fixt (repEmul τ₁) (repEmul τ₂) (S.abs (repEmul (ptarr τ₁ τ₂)) tsb) --> tsb [beta1 (S.abs (repEmul τ₁) (S.app (S.fixt (repEmul τ₁) (repEmul τ₂) (S.abs (repEmul τ₁ ⇒ repEmul τ₂) tsb[wkm↑])) (S.var 0)))]) by (refine (eval_ctx₀ S.phole _ _); constructor).
     assert (es1 : S.evaln (S.fixt (repEmul τ₁) (repEmul τ₂) (S.abs (repEmul (ptarr τ₁ τ₂)) tsb)) (tsb [beta1 (S.abs (repEmul τ₁) (S.app (S.fixt (repEmul τ₁) (repEmul τ₂) (S.abs (repEmul τ₁ ⇒ repEmul τ₂) tsb[wkm↑])) (S.var 0)))])  1) by 
         (eauto using S.evaln; omega).
     assert (es2 : forall Cu, U.ECtx Cu → U.evaln (U.pctx_app (U.ufix₁ (U.abs tub)) Cu) (U.pctx_app (tub[beta1 (U.abs (U.app (U.ufix₁ (U.abs tub[wkm↑])) (U.var 0)))]) Cu) 2) by
@@ -526,32 +541,26 @@ Section CompatibilityLemmas.
     clear es es1 es2.
 
     (* use the assumption about tsb and tub we extracted from vr *)
-    refine (bodyrel w _ _ _ _); try omega.
+    refine (hyp w _ _ _ _); try omega.
 
     (* prove valrel for values being substituted into tsb and tub *)
-    (* don't use crush cause it messes up the OfType proof for some reason *)
     rewrite -> valrel_fixp.
-    unfold valrel'; simpl.
-    split; [|crush].
+    unfold valrel', arr_rel; split; intros.
     - (* first the OfType relation *)
-      unfold OfType, OfTypeStlc, OfTypeUtlc. repeat split; [|crush].
-      econstructor; fold repEmul; econstructor; [econstructor|repeat econstructor].
-      change (S.abs _ tsb[wkm↑]) with ((S.abs (repEmul τ₁ ⇒ repEmul τ₂) tsb)[wkm]).
-      destruct ot as [[vtsb ttsb] ttub].
       crush.
     - (* prove the termrel of the body of the abstractions *)
-      refine (termrel_app _ _); [|crush].
+      refine (termrel_app (τ₁ := τ₁) (τ₂ := τ₂)_ _); crush.
       change (abs (tub[wkm↑][wkm↑][(beta1 tu')↑↑])) with ((abs tub)[wkm][wkm][(beta1 tu')↑]).
       change (S.abs _ _) with  ((S.abs (repEmul τ₁ ⇒ repEmul τ₂) tsb)[wkm][(beta1 ts')]).
-      rewrite <- apply_wkm_comm. 
+      rewrite <- apply_wkm_comm.
       rewrite -> ?apply_wkm_beta1_cancel.
       change (U.app _ _) with (U.ufix₁ (abs tub)).
       (* the goal is now what we set out to prove initially but in a strictly
            later world, so we can use the induction hypothesis from our
            well-founded induction on worlds *)
-      refine (indHyp _ _ _ _ _); try unfold ltof; crush.
+      refine (indHyp _ _ _ _ _); crush.
       (* why do I need to call crush again? *)
-      crush.
+      eapply hyp; crush.
   Qed.
   
   Lemma termrel_fix {d w τ₁ τ₂ ts tu} :
